Show that sort is sorted

examples/containers/theories/SortSorted.v
@@ -71,17 +71,6 @@ Next Obligation.
               apply IH; simpl; omega.
 Qed.
 
-Lemma ascending_permutation:
-  forall x xs (ys : list a),
-  Permutation (List.concat (ascending cmp x (app xs) ys)) (xs ++ x :: ys).
-Proof. intros. apply descending_asscending_permutation. Qed.
-
-Lemma descending_permutation:
-  forall x (xs ys : list a),
-  Permutation (List.concat (descending cmp x xs ys)) (xs ++ x :: ys).
-Proof. intros. apply descending_asscending_permutation. Qed.
-
-
 Lemma sequences_permutation:
   forall  (xs : list a), Permutation (List.concat (sequences cmp xs)) xs.
 Proof.
@@ -90,10 +79,23 @@ Proof.
   repeat destruct_match.
   * simpl. reflexivity.
   * simpl. reflexivity.
-  * apply descending_permutation.
+  * apply descending_asscending_permutation.
   * replace (fun y : list a => a0 :: y) with (app [a0]) by (simpl; reflexivity).
-    apply ascending_permutation.
+    apply descending_asscending_permutation.
 Qed.
+
+
+Lemma mergeAll_singleton: forall xs,
+  mergeAll cmp [xs] = xs.
+Proof.
+  intros.
+  unfold mergeAll at 1. unfold mergeAll_func.
+  lazymatch goal with 
+    |- Wf.Fix_sub ?A ?R ?Rwf ?P ?F_sub ?x = ?rhs => 
+    apply (@Wf.WfExtensionality.fix_sub_eq_ext A R Rwf P F_sub x)
+  end.
+Qed.
+
 
 Lemma mergeAll_eq: forall xs ys zss,
   mergeAll cmp (xs :: ys :: zss) = mergeAll cmp (mergePairs cmp (xs :: ys :: zss)).
@@ -105,6 +107,7 @@ Proof.
     apply (@Wf.WfExtensionality.fix_sub_eq_ext A R Rwf P F_sub x)
   end.
 Qed.
+
 
 Lemma merge_permutation:
   forall xs ys,
@@ -176,4 +179,207 @@ Theorem sort_permutation:
 Proof.
   intros.
   apply sortBy_permutation.
+Qed.
+
+(** ** [sort] is sorted *)
+
+Lemma LocallySorted_snoc:
+  forall a lt xs x (y : a),
+  LocallySorted lt (xs ++ [x]) ->
+  lt x y ->
+  LocallySorted lt ((xs ++ [x]) ++ [y]).
+Proof.
+  intros.
+  remember (xs ++ [x]) as ys.
+  revert xs Heqys.
+  induction H; intros xs Heqys.
+  * exfalso. eapply app_cons_not_nil. eassumption.
+  * 
+    assert (xs = []). {
+      destruct xs; try reflexivity.
+      inversion Heqys.
+      exfalso. eapply app_cons_not_nil. eassumption.
+    }
+    subst.
+    simpl in *. inversion Heqys. subst.
+    constructor. constructor. assumption.
+  * destruct xs; inversion Heqys; subst; clear Heqys.
+    specialize (IHLocallySorted _ H4).
+    destruct xs; inversion H4; subst; clear H4; simpl in *.
+    + repeat (assumption || constructor).
+    + repeat (assumption || constructor).
+Qed.
+
+Section Sorted.
+Context {a} (cmp : a -> a -> comparison).
+Context (le : a -> a -> Prop).
+
+Variable cmp_Gt_false : forall a b, (eq_comparison (cmp a b) Gt = false -> le a b).
+Variable cmp_Gt_true : forall a b, (eq_comparison (cmp a b) Gt = true -> le b a).
+
+Local Infix "<=" := le.
+
+Ltac destruct_le :=
+  lazymatch goal with |- context[eq_comparison (cmp ?x ?y) Gt] =>
+    let H := fresh "Hle" in
+    destruct (eq_comparison (cmp x y) Gt) eqn:H;
+    [ apply cmp_Gt_true in H | apply cmp_Gt_false in H ]
+  end.
+
+
+Program Fixpoint descending_asscending_sorted
+  (ys : list a) { measure (length ys) } :
+  (forall x xs, LocallySorted le (x :: xs) -> Forall (LocallySorted le) (descending cmp x xs ys)) /\
+  (forall x xs, LocallySorted le (xs ++ [x]) -> Forall (LocallySorted le) (ascending cmp x (app xs) ys)) := _.
+Next Obligation.
+  rename descending_asscending_sorted into IH.
+  destruct ys.
+  * split; intros.
+    + simpl. constructor. assumption. constructor. constructor. constructor.
+    + simpl. constructor. assumption. constructor. constructor. constructor.
+  * split; intros.
+    + simpl.
+      destruct_le.
+      - apply IH; only 1: (simpl; omega).
+        constructor; assumption.
+      - constructor. assumption.
+        destruct_match.
+        ** constructor. constructor. constructor.
+        ** destruct_le.
+           ++ apply IH; only 1: (simpl; omega).
+              constructor. constructor. assumption.
+           ++ replace (fun y : list a => a0 :: y) with (app [a0]) by (simpl; reflexivity).
+              apply IH; only 1: (simpl; omega).
+              constructor. constructor. assumption.
+    + simpl.
+      rewrite if_negb.
+      destruct_le.
+      - constructor. assumption.
+        destruct_match.
+        ** constructor. constructor. constructor.
+        ** destruct_le.
+           ++ apply IH; only 1: (simpl; omega).
+              constructor. constructor. assumption.
+           ++ replace (fun y : list a => a0 :: y) with (app [a0]) by (simpl; reflexivity).
+              apply IH; only 1: (simpl; omega).
+              constructor. constructor. assumption.
+      - replace ((fun arg_54__ : list a => xs ++ x :: arg_54__)) with (app (xs ++ [x]))
+          by (extensionality r; rewrite <- app_assoc; reflexivity).
+        apply IH; only 1: (simpl; omega).
+        apply LocallySorted_snoc; assumption.
+Qed.
+
+Lemma sequences_sorted:
+  forall  (xs : list a), Forall (LocallySorted le) (sequences cmp xs).
+Proof.
+  intros.
+  unfold sequences.
+  repeat (destruct_le || destruct_match).
+  * simpl. repeat constructor.
+  * simpl. repeat constructor.
+  * apply descending_asscending_sorted.
+    repeat (assumption || constructor).
+  * replace (fun y : list a => a0 :: y) with (app [a0]) by (simpl; reflexivity).
+    apply descending_asscending_sorted.
+    repeat (assumption || constructor).
+Qed.
+
+Lemma HdRel_Permutation:
+  forall x xs ys,
+  Permutation xs ys -> HdRel le x ys -> HdRel le x xs.
+Admitted.
+
+Lemma merge_sorted:
+  forall xs ys,
+  Sorted le xs ->
+  Sorted le ys ->
+  Sorted le (merge cmp xs ys).
+Proof.
+  intros.
+  revert ys H0.
+  induction H.
+  * destruct ys; intros; repeat (assumption || constructor).
+  * simpl.
+    intros.
+    induction H1.
+    + repeat (assumption || constructor).
+    + simpl.
+      destruct_le.
+      - constructor.
+        apply IHSorted0.
+        (* a bit ugly to do this here *)
+        clear -H2 Hle le cmp_Gt_false cmp_Gt_true.
+        induction H2.
+        ++ repeat (assumption || constructor).
+        ++ destruct_le.
+           ** repeat (assumption || constructor).
+           ** constructor. repeat (assumption || constructor). 
+      - constructor.
+        apply IHSorted.
+        constructor.
+        assumption.
+        assumption.
+        eapply HdRel_Permutation.
+        etransitivity.
+        apply merge_permutation.
+        symmetry.
+        apply Permutation_middle.
+        constructor. assumption.
+Qed.
+
+Program Fixpoint mergePairs_sorted
+  (xss : list (list a)) { measure (length xss) } :
+  Forall (Sorted le) xss -> Forall (Sorted le) (mergePairs cmp xss) := _.
+Next Obligation.
+  intros.
+  destruct xss as [|xs[|ys zss]].
+  * repeat (assumption || constructor).
+  * repeat (assumption || constructor).
+  * inversion_clear H. inversion_clear H1.
+    constructor.
+    apply merge_sorted; assumption.
+    apply mergePairs_sorted; only 1: (simpl; omega).
+    assumption.
+Qed.
+
+Program Fixpoint mergeAll_sorted
+  (xss : list (list a)) { measure (length xss) } :
+  Forall (Sorted le) xss -> Sorted le (mergeAll cmp xss) := _.
+Next Obligation.
+  destruct xss as [|xs[|ys zss]].
+  * repeat (assumption || constructor).
+  * inversion_clear H. rewrite mergeAll_singleton. assumption.
+  * rewrite mergeAll_eq.
+    apply mergeAll_sorted. {
+      pose proof (mergePairs_length (length zss) _ cmp zss xs ys).
+      apply H0.
+      omega.
+    }
+    apply mergePairs_sorted.
+    assumption.
+Qed.
+
+Lemma sortBy_sorted:
+  forall  (xs : list a), Sorted le (sortBy cmp xs).
+Proof.
+  intros.
+  unfold sortBy.
+  apply mergeAll_sorted.
+  assert (Forall (LocallySorted le) (sequences cmp xs)) by (apply sequences_sorted).
+  rewrite Forall_forall in *.
+  intros x Hx. specialize (H x Hx).
+  rewrite Sorted_LocallySorted_iff.
+  assumption.
+Qed.
+
+End Sorted.
+
+
+Theorem sort_sorted:
+  forall a `(Ord a) `(OrdLaws a) (xs : list a), Sorted (fun x y => x <= y = true) (sort xs).
+Proof.
+  intros.
+  apply sortBy_sorted.
+  * intros x y ?. destruct (compare x y) eqn:?; simpl in *; try congruence; try solve [order a].
+  * intros x y ?. destruct (compare x y) eqn:?; simpl in *; try congruence; try solve [order a].
 Qed.
